books/centaur/fgl/logicman.lisp
@@ -2712,7 +2712,8 @@ registers are not used.</p>"
     numerator rationalp realpart
     stringp symbol-name symbol-package-name
     symbolp
-    binder syntax-interp-fn abort-rewrite unequiv assume narrow-equiv fgl-interp-obj trigger-constraints conditionalize
+    binder syntax-interp-fn abort-rewrite unequiv assume-fn
+    narrow-equiv fgl-interp-obj trigger-constraints conditionalize-fn
     fgl-time-fn fgl-hide
     #+:non-standard-analysis acl2::floor1
 
